%===============================================================================
% $Id: ifacconf.tex 7 2007-11-21 12:50:23Z jpuente $
% Template for IFAC meeting papers
% Copyright (c) 2007 International Federation of Automatic Control
%===============================================================================
\documentclass{ifacconf}

\usepackage[round]{natbib} % you should have natbib.sty
\usepackage{graphicx}      % include this line if your document contains figures
\usepackage{amsmath}
\usepackage{booktabs}
%===============================================================================
\begin{document}
\begin{frontmatter}

\title{Nonlinear Control Applied to 4D Transport Aircraft Guidance} 
% Title, preferably not more than 10 words.

\thanks[footnoteinfo]{Acknowledgements go here...}

\author[First]{G. Sousa} 
%\author[Second]{Second B. Author, Jr.} 
%\author[Third]{Third C. Author}

\address[First]{Instituto Superior TÃ©cnico, Lisbon, Portugal (guilherme.sousa@ist.utl.pt
).}
%\address[Second]{Colorado State University, 
%   Fort Collins, CO 80523 USA (e-mail: author@lamar. colostate.edu)}
%\address[Third]{Electrical Engineering Department, 
%   Seoul National University, Seoul, Korea, (e-mail: author@snu.ac.kr)}

\input{ExtendedAbstract_abstr.tex}

\end{frontmatter}
%===============================================================================

\input{ExtendedAbstract_intro.tex}
\input{ExtendedAbstract_backg.tex}
\input{ExtendedAbstract_imple.tex}
\input{ExtendedAbstract_resul.tex}
\input{ExtendedAbstract_concl.tex}


\bibliography{ExtendedAbstract_ref_db}            

\appendix
 \section{$\dot{R_a}$ equation}
\label{sec:ra_dot}

\begin{gather*}
H_{11}=\dfrac{-V_a c_\alpha s_\beta  c_\beta - V_{w_y} c_\alpha c_\beta}{V_a(1+\tan^2\alpha)c^2_\alpha c^2_\beta}\\
H_{12}=\dfrac{V_a(c^2_\alpha c^2_\beta-s^2_\alpha c^2_\beta) + V_{w_x}c_\alpha c_\beta - V_{w_z}s_\alpha s_\beta}{V_a(1+\tan^2\alpha)c^2_\alpha c^2_\beta}\\
H_{13}=\dfrac{-V_a s_\alpha s_\beta  c_\beta - V_{w_y} s_\alpha c_\beta}{V_a(1+\tan^2\alpha)c^2_\alpha c^2_\beta}\\
H_{21}=\dfrac{V_a s_\alpha c_\beta + V_{w_z}}{V_a c_\beta}\\
H_{23}=-\dfrac{V_a c_\alpha c_\beta + V_{w_x}}{V_a c_\beta}\\
H_{31}=2 \left(-V_a s_\beta s_\alpha c_\beta - V_{w_x} s_\alpha c_\beta \right)\\
H_{32}=2\left( -V_{w_z} c_\alpha c_\beta + V_as_\alpha c_\beta s_\beta
 + V_{w_z}s_\beta + V_{w_x}s_\alpha c_\beta \right)\\
H_{33}=2\left(V_{w_y}c_\alpha c_\beta - V_{w_x}s_\beta\right)\\
Q_1=\dfrac{\left(\dfrac{1}{m}F_{za} + gc_\theta c_\phi - \dot{V}_{w_z} \right)c_\alpha c_\beta - \left(\dfrac{1}{m}(F_{xa} + T)-gs_\theta - \dot{V}_{w_x}\right)}{V_a(1+\tan^2\alpha)c^2_\alpha c^2_\beta}\\
Q_2=\dfrac{\dfrac{1}{m}F_{ya}+g c_\theta s_\phi-\dot{V}_{w_y}}{c_\beta}\\
Q_3=2 \left( \left(\dfrac{-1}{m}(F_{xa}+T) + g s_\theta - \dot{V}_{w_x} \right)c_\alpha c_\beta + \left( \dfrac{-1}{m}F_{ya} - \dot{V}_{w_y} \right)s_\beta \right.\\
\left. + \left(\dfrac{-1}{m}F_{za} - \dot{V}_{w_z} \right)s_\alpha c_\beta \right)
\label{eq:Ra_dot}
\end{gather*}

\end{document}
